Update grass.v
semanticを統一したので、それに合わせて

language/grass.v
@@ -1,22 +1,18 @@
-Module grass'.
+Require Import semantic_model.
 
-Section code.
-
-Inductive snip :=
-| app : nat -> nat -> snip
-| def : nat -> code -> snip
-with code :=
+(*code*)
+Inductive code :=
 | Cnil : code
-| Ccns : snip -> code -> code.
+| Ccns : snip -> code -> code
+with snip :=
+| app : nat -> nat -> snip
+| def : nat -> code -> snip.
 
-End code.
+Instance grass_code : language := {
+  code := code
+}.
 
-Notation "I ::- C" := (Ccns I C)(at level 60).
-
-Section semantic.
-
-Section machine.
-
+(*grass_machine*)
 Inductive env_one : Set :=
 | com : code -> env -> env_one
 with env : Set :=
@@ -29,45 +25,85 @@ with dmp : Set :=
 Inductive stack :=
 | Stk : code -> env -> dmp -> stack.
 
-Notation "C &&- E" := (com C E) (at level 60).
-Notation "f ::\ E" := (Ecns f E)(at level 60).
-Notation "f ::/ D" := (Dcns f D)(at level 60).
-
 Fixpoint n_th (E : env) (n : nat) : option env_one :=
 match E with
-| f ::\ E' =>
+| Ecns f E' =>
   match n with | O => Some f | S n' => n_th E' n' end
 | Enil => None
 end.
 
 Definition one_step (S:stack) : option stack :=
 match S with
-| Stk (app m n ::- C) E D =>
+| Stk (Ccns (app m n) C) E D =>
     let fn := n_th E n in
     let fm := n_th E m in
     match (fn , fm) with
-    | (Some (Cn &&- En) , Some (Cm &&- Em)) =>
-      Some (Stk Cm ((Cn &&- En) ::\ Em) ((C &&- E) ::/ D))
+    | (Some (com Cn En) , Some (com Cm Em)) =>
+      Some (Stk Cm (Ecns (com Cn En) Em) (Dcns (com C E) D))
     | (_ , _) => None
     end
-| Stk (def 0 C' ::- C) E D =>
-      Some (Stk C ((C' &&- E) ::\ E) D)
-| Stk (def (S n) C' ::- C) E D =>
-      Some (Stk C ((((def n C') ::- Cnil) &&- E) ::\ E) D)
-| Stk Cnil (f ::\ E) ((C' &&- E') ::/ D) =>
-      Some (Stk C' (f ::\ E') D)
+| Stk (Ccns (def 0 C') C) E D =>
+      Some (Stk C (Ecns (com C' E) E) D)
+| Stk (Ccns (def (S n) C') C) E D =>
+      Some (Stk C (Ecns (com (Ccns (def n C') Cnil) E) E) D)
+| Stk Cnil (Ecns f E) (Dcns (com C' E') D) =>
+      Some (Stk C' (Ecns f E') D)
 | Stk _ _ _ => None
 end.
 
-End machine.
+Definition is_stop (m :stack) : bool :=
+  match m with
+  | Stk (Ccns _ _) _ _ => false
+  | Stk  Cnil (Ecns f E) (Dcns f' D) => false
+  | Stk _ _ _ => true
+  end.
 
-Section operational_semantics.
+Definition take_value(m :stack) : forall (_ :is_stop m = true), env :=
+  (fun _:is_stop m = true =>
+  match m with
+  | Stk C E D => E
+  end).
+
+Theorem H1_stop_means :
+  forall m :stack,
+  (is_stop m = true) ->  (one_step m = None).
+Proof.
+  intros m l. destruct m. induction c.
+  - induction d;induction e.
+    { auto. } { auto. } { auto. }
+    { simpl in l. discriminate. }
+  - simpl in l. discriminate.
+Qed.
+
+Theorem H1_cor :
+  forall m :stack,
+  (is_stop m = true) -> (one_step m = Some m) \/ (one_step m = None) .
+Proof. intros. apply or_intror. apply (H1_stop_means m H). Qed.
+
+Instance grass_machine : machine := {
+  state := stack;
+  step := one_step;
+  stop_or := is_stop;
+  stop_means := H1_cor;
+}.
+
+(*grass_machine semantic*)
+
+Inductive EQ (e:env) : env -> Prop :=
+EQ_refl : EQ e e.
+Theorem EQ_ref : forall e:env, EQ e e.
+Proof. intro e. apply EQ_refl. Qed.
+Theorem EQ_sym : forall (e1 e2 :env), EQ e1 e2 -> EQ e2 e1.
+Proof. intros e1 e2 H. destruct H. apply EQ_ref. Qed.
+Theorem EQ_trs : forall (e1 e2 e3 :env),
+EQ e1 e2 /\ EQ e2 e3 -> EQ e1 e3.
+Proof. intros e1 e2 e3 H. destruct H as [H0 H1].
+destruct H0. destruct H1. apply EQ_ref. Qed.
 
 Inductive has_value : stack -> env -> Prop :=
 | HALT : forall (E : env) , has_value (Stk Cnil E Dnil) E
 | step : forall (S S': stack) (E : env),
     Some S = one_step S' -> has_value S E -> has_value S' E.
-
 
 Lemma L0:forall (E1 E2 : env), has_value (Stk Cnil E1 Dnil) E2 -> E1 = E2.
 Proof.
@@ -81,8 +117,17 @@ Qed.
 Lemma L1:forall (S:stack)(E:env), ~ Some S = one_step (Stk Cnil E Dnil).
 intros. unfold not. intro H. induction E;simpl in H;discriminate. Qed.
 
-Theorem partiality : forall (S:stack) (E1 E2:env),
-  has_value S E1 /\ has_value S E2 -> E1 = E2.
+Theorem H2_two_def_agree_if_stop :
+  forall (m :stack) (l :is_stop m = true)(v :env) ,
+  has_value m v -> take_value m l = v.
+Proof.
+  intros m l v H. destruct H.
+  - auto.
+  - rewrite (H1_stop_means S' l) in H. discriminate.
+Qed.
+
+Theorem H3_partiality : forall (m :stack) (v1 v2 :env),
+  has_value m v1 /\ has_value m v2 -> v1 = v2.
 Proof.
   intros S E1 E2 H.
   induction H as [H0 H1].
@@ -91,8 +136,37 @@ Proof.
   rewrite <- H1 in H. inversion H. subst. apply IHhas_value. apply H2.
 Qed.
 
-End operational_semantics.
+Lemma L2 :forall (e1 e2 :env), e1 = e2 -> EQ e1 e2.
+Proof. intros e1 e2 H. rewrite H. apply EQ_refl. Qed.
 
-End semantic.
+Theorem H3_cor :forall (m :stack)(_:is_halt m) (v1 v2 :env),
+  has_value m v1 /\ has_value m v2 -> EQ v1 v2.
+Proof. intros. apply L2. exact (H3_partiality m v1 v2 H0). Qed.
 
-End grass'.
+Instance ENV : value := {
+  supp := env;
+  eq := EQ;
+  eq_ref := EQ_ref;
+  eq_sym := EQ_sym;
+  eq_trs := EQ_trs;
+}.
+
+Instance grass_machine_semantic
+: machine_semantic grass_machine ENV := {
+  mchine_has_value :=
+    (fun S:state => fun _ :is_halt S => has_value S);
+  machine_partiality := H3_cor;
+}.
+
+(*code semantic*)
+
+Definition interpret (c:code)(e:env) :stack := Stk c e Dnil.
+
+Instance grass_compile 
+: language_compile grass_code grass_machine ENV := {
+  compile := interpret;
+}.
+
+Definition grass_code_semantic :=
+  operational_semantics grass_code ENV
+  grass_machine grass_machine_semantic grass_compile.
